src/HOL/IMP/Abs_Int1_ivl.thy
@@ -160,26 +160,20 @@ fun filter_less_ivl :: "bool \<Rightarrow> ivl \<Rightarrow> ivl \<Rightarrow> i
          I (max_option False (l1 + Some 1) l2) h2)
    else (I (max_option False l1 l2) h1, I l2 (min_option True h1 h2)))"
 
-interpretation Rep rep_ivl
+interpretation Val_abs rep_ivl num_ivl plus_ivl
 proof
   case goal1 thus ?case
     by(auto simp: rep_ivl_def le_ivl_def le_option_def split: ivl.split option.split if_splits)
 next
   case goal2 show ?case by(simp add: rep_ivl_def Top_ivl_def)
-qed
-
-interpretation Val_abs rep_ivl num_ivl plus_ivl
-proof
-  case goal1 thus ?case by(simp add: rep_ivl_def num_ivl_def)
 next
-  case goal2 thus ?case
+  case goal3 thus ?case by(simp add: rep_ivl_def num_ivl_def)
+next
+  case goal4 thus ?case
     by(auto simp add: rep_ivl_def plus_ivl_def split: ivl.split option.splits)
-next
-  case goal3 thus ?case
-    by(auto simp: plus_ivl_def le_ivl_def le_option_def empty_def split: if_splits ivl.splits option.splits)
 qed
 
-interpretation Rep1 rep_ivl
+interpretation Val_abs1_rep rep_ivl num_ivl plus_ivl
 proof
   case goal1 thus ?case
     by(auto simp add: rep_ivl_def meet_ivl_def empty_def min_option_def max_option_def split: ivl.split option.split)
@@ -206,23 +200,16 @@ next
   case goal2 thus ?case
     by(cases a1, cases a2,
       auto simp: rep_ivl_def min_option_def max_option_def le_option_def split: if_splits option.splits)
-next
-  case goal3 thus ?case
-    by(auto simp: filter_plus_ivl_def le_prod_def mono_meet mono_minus_ivl)
-next
-  case goal4 thus ?case
-    apply(cases a1, cases b1, cases a2, cases b2, auto simp: le_prod_def)
-    by(auto simp add: empty_def le_ivl_def le_option_def min_option_def max_option_def split: option.splits)
 qed
 
 interpretation
-  Abs_Int1 rep_ivl num_ivl plus_ivl filter_plus_ivl filter_less_ivl "(iter 20)"
+  Abs_Int1 rep_ivl num_ivl plus_ivl filter_plus_ivl filter_less_ivl
 defines afilter_ivl is afilter
 and bfilter_ivl is bfilter
 and step_ivl is step
 and AI_ivl is AI
 and aval_ivl is aval'
-proof qed (auto simp: iter_pfp strip_iter)
+proof qed
 
 definition "test1_ivl =
  ''y'' ::= N 7;
@@ -230,50 +217,78 @@ definition "test1_ivl =
  THEN ''y'' ::= Plus (V ''y'') (V ''x'')
  ELSE ''x'' ::= Plus (V ''x'') (V ''y'')"
 
-value [code] "show_acom (AI_ivl test1_ivl)"
+value [code] "show_acom_opt (AI_ivl test1_ivl)"
 
-value [code] "show_acom (AI_const test3_const)"
-value [code] "show_acom (AI_ivl test3_const)"
+value [code] "show_acom_opt (AI_const test3_const)"
+value [code] "show_acom_opt (AI_ivl test3_const)"
 
-value [code] "show_acom (AI_const test4_const)"
-value [code] "show_acom (AI_ivl test4_const)"
+value [code] "show_acom_opt (AI_const test4_const)"
+value [code] "show_acom_opt (AI_ivl test4_const)"
 
-value [code] "show_acom (AI_ivl test6_const)"
+value [code] "show_acom_opt (AI_ivl test6_const)"
 
 definition "test2_ivl =
  WHILE Less (V ''x'') (N 100)
  DO ''x'' ::= Plus (V ''x'') (N 1)"
 
-value [code] "show_acom (AI_ivl test2_ivl)"
+value [code] "show_acom_opt (AI_ivl test2_ivl)"
+value [code] "show_acom (((step_ivl \<top>)^^0) (\<bottom>\<^sub>c test2_ivl))"
+value [code] "show_acom (((step_ivl \<top>)^^1) (\<bottom>\<^sub>c test2_ivl))"
+value [code] "show_acom (((step_ivl \<top>)^^2) (\<bottom>\<^sub>c test2_ivl))"
+
+text{* Fixed point reached in 2 steps. Not so if the start value of x is known: *}
 
 definition "test3_ivl =
  ''x'' ::= N 7;
  WHILE Less (V ''x'') (N 100)
  DO ''x'' ::= Plus (V ''x'') (N 1)"
 
-value [code] "show_acom (AI_ivl test3_ivl)"
+value [code] "show_acom_opt (AI_ivl test3_ivl)"
 value [code] "show_acom (((step_ivl \<top>)^^0) (\<bottom>\<^sub>c test3_ivl))"
 value [code] "show_acom (((step_ivl \<top>)^^1) (\<bottom>\<^sub>c test3_ivl))"
 value [code] "show_acom (((step_ivl \<top>)^^2) (\<bottom>\<^sub>c test3_ivl))"
 value [code] "show_acom (((step_ivl \<top>)^^3) (\<bottom>\<^sub>c test3_ivl))"
 value [code] "show_acom (((step_ivl \<top>)^^4) (\<bottom>\<^sub>c test3_ivl))"
 
+text{* Takes as many iterations as the actual execution. Would diverge if
+loop did not terminate. Worse still, as the following example shows: even if
+the actual execution terminates, the analysis may not: *}
+
 definition "test4_ivl =
  ''x'' ::= N 0; ''y'' ::= N 100; ''z'' ::= Plus (V ''x'') (V ''y'');
  WHILE Less (V ''x'') (N 11)
  DO (''x'' ::= Plus (V ''x'') (N 1); ''y'' ::= Plus (V ''y'') (N -1))"
-value [code] "show_acom(AI_ivl test4_ivl)"
+
+text{* The value of y keeps decreasing as the analysis is iterated, no matter
+how long: *}
+
+value [code] "show_acom (((step_ivl \<top>)^^50) (\<bottom>\<^sub>c test4_ivl))"
 
 definition "test5_ivl =
  ''x'' ::= N 0; ''y'' ::= N 0;
- WHILE Less (V ''x'') (N 1001)
+ WHILE Less (V ''x'') (N 1000)
  DO (''y'' ::= V ''x''; ''x'' ::= Plus (V ''x'') (N 1))"
-value [code] "show_acom(AI_ivl test5_ivl)"
+value [code] "show_acom_opt (AI_ivl test5_ivl)"
 
-text{* Nontermination not detected: *}
+text{* Again, the analysis would not terminate: *}
 definition "test6_ivl =
  ''x'' ::= N 0;
  WHILE Less (V ''x'') (N 1) DO ''x'' ::= Plus (V ''x'') (N -1)"
-value [code] "show_acom(AI_ivl test6_ivl)"
+
+text{* Monotonicity: *}
+
+interpretation
+  Abs_Int1_mono rep_ivl num_ivl plus_ivl filter_plus_ivl filter_less_ivl
+proof
+  case goal1 thus ?case
+    by(auto simp: plus_ivl_def le_ivl_def le_option_def empty_def split: if_splits ivl.splits option.splits)
+next
+  case goal2 thus ?case
+    by(auto simp: filter_plus_ivl_def le_prod_def mono_meet mono_minus_ivl)
+next
+  case goal3 thus ?case
+    apply(cases a1, cases b1, cases a2, cases b2, auto simp: le_prod_def)
+    by(auto simp add: empty_def le_ivl_def le_option_def min_option_def max_option_def split: option.splits)
+qed
 
 end
